CookLevin/Complexity.lean
@@ -6,6 +6,7 @@ import Complexity.Complexity.Deciders.SAT_TM
 import Complexity.Complexity.Deciders.EvalCnfTM.Primitives
 import Complexity.Complexity.Deciders.EvalCnfTM.CopyUnary
 import Complexity.Complexity.Deciders.EvalCnfTM.CompareUnary
+import Complexity.Complexity.Deciders.EvalCnfTM.PerLiteral
 import Complexity.Complexity.Deciders.EvalCnfTM
 import Complexity.Complexity.Deciders.CliqueRelTM
 import Complexity.NP.SAT.CookLevin
